test/Test_Kuiper_Example_Async_Chain.cu
@@ -1,0 +1,10 @@
+#include "Kuiper_Example_Async_Chain.h"
+#include <stdint.h>
+#include <stdio.h>
+
+int main()
+{
+    uint64_t x = Kuiper_Example_Async_Chain_main();
+    printf("x = %lu\n", x);
+    return 0;
+}
