src/klas/Klas.GEMM.TensorCore2D.To.fsti
@@ -1,2 +1,0 @@
-module Klas.GEMM.TensorCore2D.To
-#lang-pulse
