src/lib/kernel/gemm/Kuiper.Kernel.GEMM.BlockTiling2D.fsti
@@ -8,6 +8,7 @@ open Kuiper.Array.Vectorized { has_vec_cpy, chunk }
 open Kuiper.Tensor
 open Kuiper.Array2.Strided
 open Kuiper.Array2.Strided.Slice
+open Kuiper.TensorRO { vtlayout_of_tlayout }
 open Kuiper.Chest
 open Kuiper.EMatrix
 module T = Kuiper.Tensor
@@ -337,8 +338,8 @@ fn gmmcomb_gpu_exact
   (#lB : layout2 k n)
   (#lC : layout2 m n)
   {| T.ctlayout lA, T.ctlayout lB, T.ctlayout lC |}
-  {| str_A : strided_row_major lA,
-     str_B : strided_row_major lB |}
+  {| str_A : strided_row_major (vtlayout_of_tlayout lA),
+     str_B : strided_row_major (vtlayout_of_tlayout lB) |}
   (#_ : squash (aligned_strided_row_major (chunk ta) str_A))
   (#_ : squash (aligned_strided_row_major (chunk tb) str_B))
   (gA : array2 ta lA { is_global gA })
@@ -441,8 +442,8 @@ fn gmmcomb_gpu_approx
   (#lB : layout2 k n)
   (#lC : layout2 m n)
   {| T.ctlayout lA, T.ctlayout lB, T.ctlayout lC |}
-  {| str_A : strided_row_major lA,
-     str_B : strided_row_major lB |}
+  {| str_A : strided_row_major (vtlayout_of_tlayout lA),
+     str_B : strided_row_major (vtlayout_of_tlayout lB) |}
   (#_ : squash (aligned_strided_row_major (chunk ta) str_A))
   (#_ : squash (aligned_strided_row_major (chunk tb) str_B))
   (gA : array2 ta lA { is_global gA })
@@ -489,6 +490,55 @@ fn gmmcomb_gpu_approx
       pure (eC' %~ MS.gmmcomb mapA_r mapB_r comb_r rC rA rB)
 
 inline_for_extraction noextract
+fn mmcomb_gpu_exact
+  (#et : Type0) {| scalar et, has_vec_cpy et |}
+  (comb : binop et)
+  (#m #n #k : szp)
+  (#lA : layout2 m k)
+  (#lB : layout2 k n)
+  (#lC : layout2 m n)
+  {| T.ctlayout lA, T.ctlayout lB, T.ctlayout lC |}
+  {| str_A : strided_row_major (vtlayout_of_tlayout lA),
+     str_B : strided_row_major (vtlayout_of_tlayout lB) |}
+  (#_ : squash (aligned_strided_row_major (chunk et) str_A))
+  (#_ : squash (aligned_strided_row_major (chunk et) str_B))
+  (gA : array2 et lA { is_global gA })
+  (#eA : chest2 et m k)
+  (gB : array2 et lB { is_global gB })
+  (#eB : chest2 et k n)
+  (gC : array2 et lC { is_global gC })
+  (#eC : chest2 et m n)
+  (bm : szp{bm /?+ m})
+  (bn : szp{bn /?+ n})
+  (bk : szp{bk /?+ k})
+  (#_ : squash (chunk et /?+ bn))
+  (#_ : squash (chunk et /?+ bk))
+  (tm : szp{tm /?+ bm})
+  (tn : szp{tn /?+ bn})
+  (#_ : squash (chunk et * (bm/tm * (bn/tn)) /?+ (bm * bk)))
+  (#_ : squash (chunk et * (bm/tm * (bn/tn)) /?+ (bk * bn)))
+  (#_ : squash (SZ.fits (bm*bk + bm/tm*(bn/tn))))
+  (#_ : squash (SZ.fits (bk*bn + bm/tm*(bn/tn))))
+  (#_: squash (SZ.fits (bm * bk) /\ SZ.fits (bk * bn)))
+  (slA : full_layout2 bm bk)
+  (slB : full_layout2 bk bn)
+  {| T.ctlayout slA, T.ctlayout slB |}
+  (#fA #fB : perm)
+  norewrite
+  preserves
+    cpu **
+    on gpu_loc (gA |-> Frac fA eA) **
+    on gpu_loc (gB |-> Frac fB eB)
+  requires
+    pure (aligned 16 (core gA)) **
+    pure (aligned 16 (core gB)) **
+    pure (m/bm * (n/bn) <= max_blocks) **
+    pure (bm/tm * (bn/tn) <= max_threads) **
+    on gpu_loc (gC |-> eC)
+  ensures
+    on gpu_loc (gC |-> MS.mmcomb comb eC eA eB)
+
+inline_for_extraction noextract
 fn mmcomb_gpu_approx
   (#et : Type0) {| scalar et, has_vec_cpy et, real_like et |}
   (comb : binop et)
@@ -498,8 +548,8 @@ fn mmcomb_gpu_approx
   (#lB : layout2 k n)
   (#lC : layout2 m n)
   {| T.ctlayout lA, T.ctlayout lB, T.ctlayout lC |}
-  {| str_A : strided_row_major lA,
-     str_B : strided_row_major lB |}
+  {| str_A : strided_row_major (vtlayout_of_tlayout lA),
+     str_B : strided_row_major (vtlayout_of_tlayout lB) |}
   (#_ : squash (aligned_strided_row_major (chunk et) str_A))
   (#_ : squash (aligned_strided_row_major (chunk et) str_B))
   (gA : array2 et lA { is_global gA })
