src/lib/kernel/gemm/Kuiper.Kernel.GEMM.TensorCore.fsti
@@ -8,6 +8,7 @@ open Kuiper.EMatrix
 open Kuiper.Array.Vectorized { has_vec_cpy, chunk }
 
 open Kuiper.Array2.Strided
+open Kuiper.TensorRO { vtlayout_of_tlayout }
 open Kuiper.Tensor.Layout.Alg { l2_row_major as rm }
 open Kuiper.TensorCore
 
@@ -19,10 +20,10 @@ val mk_kernel
   (#et_ab #et_c : Type0)
   {| scalar et_ab, has_vec_cpy et_ab, scalar et_c |}
   (#m #n #k : szp)
-  (#lA : layout2 m k) {| T.ctlayout lA, str_A : strided_row_major lA |}
+  (#lA : layout2 m k) {| T.ctlayout lA, str_A : strided_row_major (vtlayout_of_tlayout lA) |}
   (gA : array2 et_ab lA { is_global gA })
   (#eA : chest2 et_ab m k)
-  (#lB : layout2 k n) {| T.ctlayout lB, str_B : strided_row_major lB |}
+  (#lB : layout2 k n) {| T.ctlayout lB, str_B : strided_row_major (vtlayout_of_tlayout lB) |}
   (#_ : squash (aligned_strided_row_major (chunk et_ab) str_A))
   (#_ : squash (aligned_strided_row_major (chunk et_ab) str_B))
   (gB : array2 et_ab lB { is_global gB })
